DomainSemantics/Strong.lean
@@ -7,20 +7,17 @@ open VExpr
 
 section
 set_option hygiene false
-
 section
 local notation:65 Γ " ⊢ " e " : " A:30 => IsDefEqStrong env uvars Γ e e A
 local notation:65 Γ " ⊢ " e1 " ≡ " e2 " : " A:30 => IsDefEqStrong env uvars Γ e1 e2 A
 
-inductive IsDefEqStrong (env : VEnv) (uvars : Nat) :
-    List VExpr → VExpr → VExpr → VExpr → Prop where
+inductive IsDefEqStrong (env : VEnv) (uvars : Nat) : List VExpr → VExpr → VExpr → VExpr → Prop where
   | bvar : Lookup Γ i A → Γ ⊢ A : .sort u → Γ ⊢ .bvar i : A
   | symm : Γ ⊢ e ≡ e' : A → Γ ⊢ e' ≡ e : A
   | trans : Γ ⊢ e₁ ≡ e₂ : A → Γ ⊢ e₂ ≡ e₃ : A → Γ ⊢ e₁ ≡ e₃ : A
-  | sortDF : Γ ⊢ .sort l ≡ .sort l : .sort true
+  | sortDF : Γ ⊢ .sort l : .sort true
   | appDF :
     Γ ⊢ A : .sort u →
-    A::Γ ⊢ B : .sort v →
     Γ ⊢ f ≡ f' : .forallE A B →
     Γ ⊢ a ≡ a' : A →
     Γ ⊢ B.inst a ≡ B.inst a' : .sort v →
@@ -28,7 +25,6 @@ inductive IsDefEqStrong (env : VEnv) (uvars : Nat) :
   | lamDF :
     Γ ⊢ A ≡ A' : .sort u →
     A::Γ ⊢ B : .sort v →
-    A'::Γ ⊢ B : .sort v →
     A::Γ ⊢ body ≡ body' : B →
     A'::Γ ⊢ body ≡ body' : B →
     Γ ⊢ .lam A body ≡ .lam A' body' : .forallE A B
@@ -37,63 +33,20 @@ inductive IsDefEqStrong (env : VEnv) (uvars : Nat) :
     A::Γ ⊢ body ≡ body' : .sort v →
     A'::Γ ⊢ body ≡ body' : .sort v →
     Γ ⊢ .forallE A body ≡ .forallE A' body' : .sort v
-  | defeqDF :
-    Γ ⊢ A ≡ B : .sort u → Γ ⊢ e1 ≡ e2 : A → Γ ⊢ e1 ≡ e2 : B
+  | defeqDF : Γ ⊢ A ≡ B : .sort u → Γ ⊢ e1 ≡ e2 : A → Γ ⊢ e1 ≡ e2 : B
   | beta :
-    Γ ⊢ A : .sort u → A::Γ ⊢ B : .sort v →
-    A::Γ ⊢ e : B → Γ ⊢ e' : A →
-    Γ ⊢ B.inst e' : .sort v →
+    Γ ⊢ A : .sort u → A::Γ ⊢ e : B → Γ ⊢ e' : A →
+    Γ ⊢ .app (.lam A e) e' : B.inst e' →
     Γ ⊢ e.inst e' : B.inst e' →
     Γ ⊢ .app (.lam A e) e' ≡ e.inst e' : B.inst e'
   | eta :
-    Γ ⊢ A : .sort u →
-    A::Γ ⊢ B : .sort v →
-    A.lift::A::Γ ⊢ B.liftN 1 1 : .sort v →
     Γ ⊢ e : .forallE A B →
-    A::Γ ⊢ e.lift : .forallE A.lift (B.liftN 1 1) →
-    A::Γ ⊢ A.lift : .sort u →
+    Γ ⊢ .lam A (.app e.lift (.bvar 0)) : .forallE A B →
     Γ ⊢ .lam A (.app e.lift (.bvar 0)) ≡ e : .forallE A B
   | proofIrrel :
     Γ ⊢ p : .sort false → Γ ⊢ h : p → Γ ⊢ h' : p →
     Γ ⊢ h ≡ h' : p
 
-end
-
-section
-variable (env : VEnv) (uvars : Nat)
-local notation:65 Γ " ⊢ " e " : " A:30 => HasTypeStrong env uvars Γ e A true
-local notation:65 Γ " ⊢ " e " :! " A:30 => HasTypeStrong env uvars Γ e A false
-local notation:65 Γ " ⊢ " e1 " ≡ " e2 " : " A:30 => IsDefEqStrong env uvars Γ e1 e2 A
-
-/--
-This is functionally a mutual inductive type,
-but using a bool index makes it easier to do induction in lean.
-The defeq rule is separated from the structural rules for easy inversion.
--/
-inductive HasTypeStrong : List VExpr → VExpr → VExpr → Bool → Prop where
-  | bvar : Lookup Γ i A → Γ ⊢ A : .sort u → Γ ⊢ .bvar i :! A
-  | sort' : Γ ⊢ .sort l :! .sort true
-  | app :
-    Γ ⊢ A : .sort u →
-    A::Γ ⊢ B : .sort v →
-    Γ ⊢ .forallE A B : .sort v →
-    Γ ⊢ f : .forallE A B →
-    Γ ⊢ a : A →
-    Γ ⊢ B.inst a : .sort v →
-    Γ ⊢ .app f a :! B.inst a
-  | lam :
-    Γ ⊢ A : .sort u →
-    A::Γ ⊢ B : .sort v →
-    A::Γ ⊢ body : B →
-    Γ ⊢ .forallE A B : .sort v →
-    Γ ⊢ .lam A body :! .forallE A B
-  | forallE :
-    Γ ⊢ A : .sort u →
-    A::Γ ⊢ body : .sort v →
-    Γ ⊢ .forallE A body :! .sort v
-  | base : Γ ⊢ e :! A → Γ ⊢ e : A
-  | defeq : Γ ⊢ A ≡ B : .sort u →
-    Γ ⊢ A : .sort u → Γ ⊢ B : .sort u → Γ ⊢ e : A → Γ ⊢ e : B
 end
 
 end
@@ -111,28 +64,22 @@ theorem IsDefEqStrong.weakN (W : Ctx.LiftN n k Γ Γ') (H : env.IsDefEqStrong U 
   | symm _ ih => exact .symm (ih W)
   | trans _ _ ih1 ih2 => exact .trans (ih1 W) (ih2 W)
   | sortDF => exact .sortDF
-  | appDF _ _ _ _ _ ih1 ih2 ih3 ih4 ih5 =>
-    refine liftN_inst_hi .. ▸ .appDF (ih1 W) (ih2 W.succ) (ih3 W) (ih4 W) ?_
-    exact liftN_inst_hi .. ▸ liftN_inst_hi .. ▸ ih5 W
-  | lamDF _ _ _ _ _ ih1 ih2 ih3 ih4 ih5 =>
-    exact .lamDF (ih1 W) (ih2 W.succ) (ih3 W.succ) (ih4 W.succ) (ih5 W.succ)
+  | appDF _ _ _ _ ih1 ih2 ih3 ih4 =>
+    exact liftN_inst_hi .. ▸ .appDF (ih1 W) (ih2 W) (ih3 W)
+      (liftN_inst_hi .. ▸ liftN_inst_hi .. ▸ ih4 W)
+  | lamDF _ _ _ _ ih1 ih2 ih3 ih4 =>
+    exact .lamDF (ih1 W) (ih2 W.succ) (ih3 W.succ) (ih4 W.succ)
   | forallEDF _ _ _ ih1 ih2 ih3 => exact .forallEDF (ih1 W) (ih2 W.succ) (ih3 W.succ)
   | defeqDF _ _ ih1 ih2 => exact .defeqDF (ih1 W) (ih2 W)
-  | beta _ _ _ _ _ _ ih1 ih2 ih3 ih4 ih5 ih6 =>
+  | beta _ _ _ _ _ ih1 ih2 ih3 ih4 ih5 =>
     refine liftN_inst_hi .. ▸ liftN_instN_hi .. ▸ .beta
-      (ih1 W) (ih2 W.succ) (ih3 W.succ) (ih4 W)
-      (liftN_instN_hi .. ▸ ih5 W :)
-      (liftN_instN_hi .. ▸ liftN_instN_hi .. ▸ ih6 W :)
-  | @eta Γ a u B v e _ _ _ _ _ _ ih1 ih2 ih3 ih4 ih5 ih6 =>
-    have := IsDefEqStrong.eta (ih1 W) (ih2 W.succ) ?_ (ih4 W) ?_ ?_
+      (ih1 W) (ih2 W.succ) (ih3 W)
+      (liftN_instN_hi .. ▸ ih4 W :)
+      (liftN_instN_hi .. ▸ liftN_instN_hi .. ▸ ih5 W :)
+  | @eta Γ e A B _ _ ih2 ih3 =>
+    have := IsDefEqStrong.eta (ih2 W) ?_
     · simp [liftN]; rwa [← lift_liftN']
-    · specialize ih3 W.succ.succ
-      have := liftN'_comm B n 1 (k+1) 1 (Nat.le_add_left ..)
-      rw [Nat.add_comm 1] at this; rwa [← this, ← lift_liftN'] at ih3
-    · have ih5 : IsDefEqStrong _ _ _ _ _ (liftN n (lift (forallE ..)) _) := ih5 W.succ
-      rwa [← lift_liftN', ← lift_liftN'] at ih5
-    · have ih6 := ih6 W.succ
-      rwa [← lift_liftN'] at ih6
+    · specialize ih3 W; simp [liftN] at ih3; rwa [← lift_liftN'] at ih3
   | proofIrrel _ _ _ ih1 ih2 ih3 => exact .proofIrrel (ih1 W) (ih2 W) (ih3 W)
 
 theorem IsDefEqStrong.defeq (H : IsDefEqStrong env U Γ e1 e2 A) : env.IsDefEq U Γ e1 e2 A := by
@@ -141,12 +88,12 @@ theorem IsDefEqStrong.defeq (H : IsDefEqStrong env U Γ e1 e2 A) : env.IsDefEq U
   | symm _ ih => exact .symm ih
   | trans _ _ ih1 ih2 => exact .trans ih1 ih2
   | sortDF => exact .sortDF
-  | appDF _ _ _ _ _ _ _ ih1 ih2 => exact .appDF ih1 ih2
-  | lamDF _ _ _ _ _ ih1 _ _ ih2 => exact .lamDF ih1 ih2
-  | forallEDF _ _ _ ih1 ih2 => exact .forallEDF ih1 ih2
+  | appDF _ _ _ _ _ ih1 ih2 _ => exact .appDF ih1 ih2
+  | lamDF _ _ _ _ ih1 _ ih2 _ => exact .lamDF ih1 ih2
+  | forallEDF _ _ _ ih1 ih2 _ => exact .forallEDF ih1 ih2
   | defeqDF _ _ ih1 ih2 => exact .defeqDF ih1 ih2
-  | beta _ _ _ _ _ _ _ _ ih1 ih2 => exact .beta ih1 ih2
-  | eta _ _ _ _ _ _ _ _ _ ih => exact .eta ih
+  | beta _ _ _ _ _ _ ih1 ih2 _ _ => exact .beta ih1 ih2
+  | eta  _ _ ih => exact .eta ih
   | proofIrrel _ _ _ ih1 ih2 ih3 => exact .proofIrrel ih1 ih2 ih3
 
 variable! {env env' : VEnv} (henv : env ≤ env') in
@@ -157,12 +104,12 @@ theorem IsDefEqStrong.mono
   | symm _ ih => exact .symm ih
   | trans _ _ ih1 ih2 => exact .trans ih1 ih2
   | sortDF => exact .sortDF
-  | appDF _ _ _ _ _ ih1 ih2 ih3 ih4 ih5 => exact .appDF ih1 ih2 ih3 ih4 ih5
-  | lamDF _ _ _ _ _ ih1 ih2 ih3 ih4 ih5 => exact .lamDF ih1 ih2 ih3 ih4 ih5
+  | appDF _ _ _ _ ih1 ih2 ih3 ih4 => exact .appDF ih1 ih2 ih3 ih4
+  | lamDF _ _ _ _ ih1 ih2 ih3 ih4 => exact .lamDF ih1 ih2 ih3 ih4
   | forallEDF _ _ _ ih1 ih2 ih3 => exact .forallEDF ih1 ih2 ih3
   | defeqDF _ _ ih1 ih2 => exact .defeqDF ih1 ih2
-  | beta _ _ _ _ _ _ ih1 ih2 ih3 ih4 ih5 ih6 => exact .beta ih1 ih2 ih3 ih4 ih5 ih6
-  | eta _ _ _ _ _ _ ih1 ih2 ih3 ih4 ih5 ih6 => exact .eta ih1 ih2 ih3 ih4 ih5 ih6
+  | beta _ _ _ _ _ ih1 ih2 ih3 ih4 ih5 => exact .beta ih1 ih2 ih3 ih4 ih5
+  | eta _ _ ih1 ih2 => exact .eta ih1 ih2
   | proofIrrel _ _ _ ih1 ih2 ih3 => exact .proofIrrel ih1 ih2 ih3
 
 variable! {env : VEnv} in
@@ -175,99 +122,71 @@ theorem IsDefEqStrong.weak0 (H : env.IsDefEqStrong U [] e1 e2 A) :
 def CtxStrong (env : VEnv) (U Γ) :=
   OnCtx Γ fun Γ A => ∃ u, env.IsDefEqStrong U Γ A A (.sort u)
 
-variable! (henv : Ordered env) in
 nonrec theorem CtxStrong.lookup {Γ} (H : CtxStrong env U Γ) (h : Lookup Γ i A) :
     ∃ u, env.IsDefEqStrong U Γ A A (.sort u) :=
-  H.lookup h fun ⟨_, h⟩ => ⟨_, h.weakN henv .one⟩
+  H.lookup h fun ⟨_, h⟩ => ⟨_, h.weakN .one⟩
 
 theorem CtxStrong.defeq {Γ} (H : CtxStrong env U Γ) : OnCtx Γ (env.IsType U) :=
   H.mono fun ⟨_, h⟩ => ⟨_, h.defeq⟩
 
-theorem CtxStrong.levelWF : ∀ {Γ}, CtxStrong env U Γ → OnCtx Γ fun _ A => A.LevelWF U
-  | [], h => h
-  | _::_, ⟨h1, _, h2⟩ => ⟨levelWF h1, (h2.defeq.levelWF (levelWF h1)).1⟩
-
-variable! (henv : Ordered env) (h₀ : env.IsDefEqStrong U Γ₀ e₀ e₀ A₀) (hΓ₀ : CtxStrong env U Γ₀) in
+variable! {env : VEnv} (h₀ : env.IsDefEqStrong U Γ₀ e₀ e₀ A₀) (hΓ₀ : CtxStrong env U Γ₀) in
 theorem IsDefEqStrong.instN (W : Ctx.InstN Γ₀ e₀ A₀ k Γ₁ Γ) (H : env.IsDefEqStrong U Γ₁ e1 e2 A)
     (hΓ : CtxStrong env U Γ) :
     env.IsDefEqStrong U Γ (e1.inst e₀ k) (e2.inst e₀ k) (A.inst e₀ k) := by
   induction H generalizing Γ k with
-  | @bvar _ i ty _ h _ h2 ih =>
+  | @bvar _ i ty _ h h2 ih =>
     dsimp [inst]; clear h2 ih
     induction W generalizing i ty with
     | zero =>
       cases h with simp [inst_lift]
       | zero => exact h₀
       | succ h =>
-        let ⟨u, hty⟩ := hΓ₀.lookup henv h
-        exact .bvar h (hty.defeq.sort_r henv hΓ₀.defeq) hty
+        let ⟨u, hty⟩ := hΓ₀.lookup h
+        exact .bvar h hty
     | succ _ ih =>
       cases h with (simp; rw [Nat.add_comm, ← liftN_instN_lo (hj := Nat.zero_le _)])
       | zero =>
-        let ⟨u, hty⟩ := hΓ.lookup henv .zero
-        exact .bvar .zero (hty.defeq.sort_r henv hΓ.defeq) hty
-      | succ h => exact (ih h hΓ.1).weakN henv .one
+        let ⟨u, hty⟩ := hΓ.lookup .zero
+        exact .bvar .zero hty
+      | succ h => exact (ih h hΓ.1).weakN .one
   | symm _ ih => exact .symm (ih W hΓ)
   | trans _ _ ih1 ih2 => exact .trans (ih1 W hΓ) (ih2 W hΓ)
-  | sortDF h1 h2 h3 => exact .sortDF h1 h2 h3
-  | constDF h1 h2 h3 h4 h5 h6 h7 _ _ ih2 =>
-    simp [(henv.closedC h1).instL.instN_eq (Nat.zero_le _)] at ih2 ⊢
-    exact .constDF h1 h2 h3 h4 h5 h6 h7 (ih2 W hΓ)
-  | appDF h1 h2 _ _ _ _ _ ih1 ih2 ih3 ih4 ih5 =>
-    exact inst0_inst_hi .. ▸ .appDF h1 h2
-      (ih1 W hΓ) (ih2 W.succ ⟨hΓ, _, ih1 W hΓ⟩)
-      (ih3 W hΓ) (ih4 W hΓ) (inst0_inst_hi .. ▸ inst0_inst_hi .. ▸ ih5 W hΓ)
-  | lamDF h1 h2 _ _ _ _ _ ih1 ih2 ih3 ih4 ih5 =>
+  | sortDF => exact .sortDF
+  | appDF _ _ _ _ ih1 ih2 ih3 ih4 =>
+    exact inst0_inst_hi .. ▸ .appDF
+      (ih1 W hΓ) (ih2 W hΓ) (ih3 W hΓ)
+      (inst0_inst_hi .. ▸ inst0_inst_hi .. ▸ ih4 W hΓ)
+  | lamDF _ _ _ _ ih1 ih2 ih3 ih4 =>
     exact
       have hΓ' := ⟨hΓ, _, (ih1 W hΓ).hasType.1⟩
       have hΓ'' := ⟨hΓ, _, (ih1 W hΓ).hasType.2⟩
-      .lamDF h1 h2 (ih1 W hΓ) (ih2 W.succ hΓ') (ih3 W.succ hΓ'') (ih4 W.succ hΓ') (ih5 W.succ hΓ'')
-  | forallEDF h1 h2 _ _ _ ih1 ih2 ih3 =>
-    exact .forallEDF h1 h2 (ih1 W hΓ)
+      .lamDF (ih1 W hΓ) (ih2 W.succ hΓ') (ih3 W.succ hΓ') (ih4 W.succ hΓ'')
+  | forallEDF _ _ _ ih1 ih2 ih3 =>
+    exact .forallEDF (ih1 W hΓ)
       (ih2 W.succ ⟨hΓ, _, (ih1 W hΓ).hasType.1⟩) (ih3 W.succ ⟨hΓ, _, (ih1 W hΓ).hasType.2⟩)
-  | defeqDF h1 _ _ ih1 ih2 => exact .defeqDF h1 (ih1 W hΓ) (ih2 W hΓ)
-  | beta h1 h2 _ _ _ _ _ _ ih1 ih2 ih3 ih4 ih5 ih6 =>
+  | defeqDF _ _ ih1 ih2 => exact .defeqDF (ih1 W hΓ) (ih2 W hΓ)
+  | beta _ _ _ _ _ ih1 ih3 ih4 ih5 ih6 =>
     rw [inst0_inst_hi, inst0_inst_hi]; exact
       have hΓ' := ⟨hΓ, _, ih1 W hΓ⟩
-      .beta h1 h2
-        (ih1 W hΓ) (ih2 W.succ hΓ') (ih3 W.succ hΓ') (ih4 W hΓ)
+      .beta (ih1 W hΓ) (ih3 W.succ hΓ') (ih4 W hΓ)
         (inst0_inst_hi .. ▸ ih5 W hΓ) (inst0_inst_hi .. ▸ inst0_inst_hi .. ▸ ih6 W hΓ)
-  | eta h1 h2 _ _ _ _ _ _ ih1 ih2 ih3 ih4 ih5 ih6 =>
-    have :=
-      have hΓ' := ⟨hΓ, _, (ih1 W hΓ).hasType.1⟩
-      IsDefEqStrong.eta h1 h2 (ih1 W hΓ) (ih2 W.succ hΓ')
-        (by
-          have := ih3 W.succ.succ ⟨hΓ', _, by
-            rw [← lift_instN_lo]; exact (ih1 W hΓ).hasType.1.weakN henv .one⟩
-          rwa [lift_instN_lo, liftN_instN_lo (hj := Nat.le_add_left ..), Nat.add_comm 1])
-        (ih4 W hΓ)
-        (by
-          have := ih5 W.succ hΓ'
-          simp only [inst, ← lift_instN_lo] at this
-          rwa [liftN_instN_lo (hj := Nat.le_add_left ..), Nat.add_comm 1])
-        (by simpa [inst, ← lift_instN_lo] using ih6 W.succ hΓ')
+  | eta _ _ ih1 ih2 =>
+    have := IsDefEqStrong.eta (ih1 W hΓ)
+      (by simpa [inst, ← lift_instN_lo] using ih2 W hΓ)
     rw [lift, liftN_instN_lo (hj := Nat.zero_le _), Nat.add_comm] at this
     simpa [inst]
   | proofIrrel _ _ _ ih1 ih2 ih3 => exact .proofIrrel (ih1 W hΓ) (ih2 W hΓ) (ih3 W hΓ)
-  | extra h1 h2 h3 h4 h5 h6 h7 _ _ _ _ _ ih4 ih5 =>
-    have ⟨⟨hA1, _⟩, hA2, hA3⟩ := henv.closed.2 h1
-    simp [
-      hA1.instL.instN_eq (Nat.zero_le _),
-      hA2.instL.instN_eq (Nat.zero_le _),
-      hA3.instL.instN_eq (Nat.zero_le _)] at ih4 ih5 ⊢
-    exact .extra h1 h2 h3 h4 h5 h6 h7 (ih4 W hΓ) (ih5 W hΓ)
 
-theorem IsDefEqStrong.defeqDF_l (henv : Ordered env) (hΓ : CtxStrong env U Γ)
+theorem IsDefEqStrong.defeqDF_l {env : VEnv} (hΓ : CtxStrong env U Γ)
     (h1 : env.IsDefEqStrong U Γ A A' (.sort u))
     (h2 : env.IsDefEqStrong U (A::Γ) e1 e2 B) : env.IsDefEqStrong U (A'::Γ) e1 e2 B := by
   simpa [instN_bvar0] using
-    have hu := h1.defeq.sort_r henv hΓ.defeq
     have hΓ' := ⟨hΓ, _, h1.hasType.2⟩
-    h1.weakN henv (.one (A := A'))
-      |>.symm.defeqDF hu (.bvar .zero hu (h1.hasType.2.weakN henv .one))
-      |>.instN henv hΓ' .zero (h2.weakN henv (.succ (.one (A := A')))) hΓ'
+    h1.weakN (.one (A := A'))
+      |>.symm.defeqDF (.bvar .zero (h1.hasType.2.weakN .one))
+      |>.instN hΓ' .zero (h2.weakN (.succ (.one (A := A')))) hΓ'
 
-variable! (henv : Ordered env) (envIH : env.OnTypes (EnvStrong env)) in
+variable! {env : VEnv} in
 theorem IsDefEqStrong.forallE_inv' (hΓ : CtxStrong env U Γ)
     (H : env.IsDefEqStrong U Γ e1 e2 V) (eq : e1 = A.forallE B ∨ e2 = A.forallE B) :
     (∃ u, env.IsDefEqStrong U Γ A A (.sort u)) ∧ ∃ v, env.IsDefEqStrong U (A::Γ) B B (.sort v) := by
@@ -278,12 +197,12 @@ theorem IsDefEqStrong.forallE_inv' (hΓ : CtxStrong env U Γ)
     obtain eq | eq := eq
     · exact ih1 hΓ (.inl eq)
     · exact ih2 hΓ (.inr eq)
-  | forallEDF _ _ h1 h2 =>
+  | forallEDF h1 h2 _ =>
     obtain ⟨⟨⟩⟩ | ⟨⟨⟩⟩ := eq
     · exact ⟨⟨_, h1.hasType.1⟩, _, h2.hasType.1⟩
-    · exact ⟨⟨_, h1.hasType.2⟩, _, h1.defeqDF_l henv hΓ h2.hasType.2⟩
-  | defeqDF _ _ _ _ ih2 => exact ih2 hΓ eq
-  | @beta _ _ _ _ _ e _ _ _ h1 _ _ h4 _ _ _ _ ih3 ih4 =>
+    · exact ⟨⟨_, h1.hasType.2⟩, _, h1.defeqDF_l hΓ h2.hasType.2⟩
+  | defeqDF _ _ _ ih2 => exact ih2 hΓ eq
+  | @beta _ _ _ e _ _ h1 _ he' _ _ _ ih3 ih4 _ _ =>
     obtain ⟨⟨⟩⟩ | eq := eq
     cases e with
     | bvar i =>
@@ -292,64 +211,37 @@ theorem IsDefEqStrong.forallE_inv' (hΓ : CtxStrong env U Γ)
     | forallE A B =>
       cases eq
       let ⟨⟨_, A1⟩, _, A2⟩ := ih3 ⟨hΓ, _, h1⟩ (.inl rfl)
-      refine ⟨⟨_, h4.instN henv hΓ .zero A1 hΓ⟩, _, h4.instN henv hΓ (.succ .zero) A2 ?_⟩
-      exact ⟨hΓ, _, h4.instN henv hΓ .zero A1 hΓ⟩
+      refine ⟨⟨_, he'.instN hΓ .zero A1 hΓ⟩, _, he'.instN hΓ (.succ .zero) A2 ?_⟩
+      exact ⟨hΓ, _, he'.instN hΓ .zero A1 hΓ⟩
     | _ => cases eq
-  | eta _ _ _ _ _ _ _ _ _ _ _ ih =>
+  | eta _ _ ih _ =>
     obtain ⟨⟨⟩⟩ | eq := eq
-    exact ih hΓ (.inl eq)
-  | @extra df ls _ Γ h1 h2 =>
-    suffices ∀ e, VExpr.instL ls e = VExpr.forallE A B →
-        EnvStrong env df.uvars e df.type →
-        (∃ u, IsDefEqStrong env U Γ A A (.sort u)) ∧
-        (∃ u, IsDefEqStrong env U (A :: Γ) B B (.sort u)) by
-      have ⟨A1, A2⟩ := envIH.2 h1
-      cases eq <;> exact this _ ‹_› ‹_›
-    intro e eq IH
-    cases e <;> cases eq; rename_i A B
-    let ⟨⟨_, A1⟩, v, A2⟩ := IH.2.2.2 _ _ rfl
-    refine ⟨⟨_, (A1.instL h2).weak0 henv⟩, v.inst ls, ?_⟩
-    have := (A2.instL h2).weakN henv (.succ (.zero Γ))
-    have C1 := (A1.instL h2).defeq.closedN henv ⟨⟩
-    have C2 := (A2.instL h2).defeq.closedN henv ⟨⟨⟩, C1⟩
-    rw [C1.liftN_eq (Nat.zero_le _), C2.liftN_eq (by exact Nat.le_refl _)] at this
-    simpa [liftN]
+    exact ih hΓ (.inr eq)
   | _ => nomatch eq
 
-variable! (henv : Ordered env) (envIH : env.OnTypes (EnvStrong env)) in
+variable! {env : VEnv} in
 theorem IsDefEqStrong.isType' (hΓ : CtxStrong env U Γ) (H : env.IsDefEqStrong U Γ e1 e2 A) :
     ∃ u, env.IsDefEqStrong U Γ A A (.sort u) := by
   induction H with
-  | bvar h => exact hΓ.lookup henv h
+  | bvar h _ => exact hΓ.lookup h
   | symm _ ih => exact ih hΓ
-  | trans _ _ ih1 => exact ih1 hΓ
-  | sortDF h1 => exact ⟨_, .sortDF h1 h1 rfl⟩
-  | constDF h1 h2 =>
-    let ⟨_, h⟩ := envIH.1 h1
-    exact ⟨_, (h.1.instL h2).weak0 henv⟩
-  | appDF _ _ _ _ _ h4 _ _ _ ih3 =>
-    let ⟨_, ih3⟩ := ih3 hΓ
-    have ⟨_, _, ih3⟩ := ih3.forallE_inv' henv envIH hΓ (.inl rfl)
-    exact ⟨_, h4.hasType.1.instN henv hΓ .zero ih3 hΓ⟩
-  | lamDF h1 h2 h3 h4 => exact ⟨_, .forallEDF h1 h2 h3.hasType.1 h4 h4⟩
-  | forallEDF h1 h2 => exact ⟨_, .sortDF ⟨h1, h2⟩ ⟨h1, h2⟩ rfl⟩
-  | defeqDF _ h2 => exact ⟨_, h2.hasType.2⟩
-  | beta _ _ _ h4 _ h6 => exact ⟨_, h6.hasType.1.instN henv hΓ .zero h4 hΓ⟩
-  | eta _ _ _ _ _ _ _ _ _ _ _ ih => exact ih hΓ
-  | proofIrrel h1 => exact ⟨_, h1⟩
-  | extra h1 h2 =>
-    have ⟨_, h⟩ := (envIH.2 h1).2.2.1
-    exact ⟨_, (h.instL h2).weak0 henv⟩
+  | trans _ _ ih1 _ => exact ih1 hΓ
+  | sortDF => exact ⟨_, .sortDF⟩
+  | appDF _ _ _ h4 _ _ _ _ => exact ⟨_, h4.hasType.1⟩
+  | lamDF h1 h2 _ _ => exact ⟨_, .forallEDF h1.hasType.1 h2 h2⟩
+  | forallEDF => exact ⟨_, .sortDF⟩
+  | defeqDF h1 _ _ _ => exact ⟨_, h1.hasType.2⟩
+  | beta _ _ _ _ _ _ _ _ ih
+  | eta _ _ ih => exact ih hΓ
+  | proofIrrel h1 _ _ _ _ _ => exact ⟨_, h1⟩
 
-theorem IsDefEqStrong.instDF
-    (henv : Ordered env) (hΓ : CtxStrong env U Γ) (hu : u.WF U) (hv : v.WF U)
+theorem IsDefEqStrong.instDF {env : VEnv} (hΓ : CtxStrong env U Γ)
     (hA : env.IsDefEqStrong U Γ A A (.sort u))
     (hB : env.IsDefEqStrong U (A::Γ) B B (.sort v))
     (hf : env.IsDefEqStrong U (A::Γ) f f' B)
     (ha : env.IsDefEqStrong U Γ a a' A) :
     env.IsDefEqStrong U Γ (f.inst a) (f'.inst a') (B.inst a) :=
   have H2 {f f' B v}
-      (hv : v.WF U)
       (hB : env.IsDefEqStrong U (A::Γ) B B (.sort v))
       (hf : env.IsDefEqStrong U (A::Γ) f f' B)
       (hi : IsDefEqStrong env U Γ (inst B a) (inst B a') (sort v)) :
@@ -358,405 +250,107 @@ theorem IsDefEqStrong.instDF
         (hf : env.IsDefEqStrong U (A::Γ) f f' B)
         (ha : IsDefEqStrong env U Γ a a A) :
         env.IsDefEqStrong U Γ (.app (.lam A f) a) (f.inst a) (B.inst a) :=
-      IsDefEqStrong.beta hu hv hA hB hf.hasType.1 ha
-        (ha.hasType.1.instN henv hΓ .zero hB hΓ)
-        (ha.hasType.1.instN henv hΓ .zero hf.hasType.1 hΓ)
+      IsDefEqStrong.beta hA hf.hasType.1 ha
+        (.appDF hA (.lamDF hA hB hf.hasType.1 hf.hasType.1) ha
+          (ha.hasType.1.instN hΓ .zero hB hΓ))
+        (ha.hasType.1.instN hΓ .zero hf.hasType.1 hΓ)
     (H1 hf ha.hasType.1).symm.trans <|
-      .trans (.appDF hu hv hA hB (.lamDF hu hv hA hB hB hf hf) ha hi) <|
-      .defeqDF hv (.symm hi) (H1 hf.hasType.2 ha.hasType.2)
-  H2 hv hB hf <| H2 (v := v.succ) hv (.sortDF hv hv rfl) hB (.sortDF hv hv rfl)
+      .trans (.appDF hA (.lamDF hA hB hf hf) ha hi) <|
+      .defeqDF (.symm hi) (H1 hf.hasType.2 ha.hasType.2)
+  H2 hB hf <| H2 .sortDF hB .sortDF
 
-variable! (henv : Ordered env) (envIH : env.OnTypes (EnvStrong env))
-  (W : CtxStrong env U Γ) in
-theorem EqUpToLevels.defeq (H : env.IsDefEqStrong U Γ e1 e2 A)
-    (H1 : EqUpToLevels U e1 e1') (H2 : EqUpToLevels U e2 e2') :
-    env.IsDefEqStrong U Γ e1' e2' A := by
-  induction H generalizing e1' e2' with
-  | bvar h1 h2 h3 => let .bvar := H1; let .bvar := H2; exact .bvar h1 h2 h3
-  | constDF h1 h2 h3 h4 h5 h6 _ _ ih1 ih2 =>
-    let .const a1 a2 a3 := H1
-    let .const b1 b2 b3 := H2
-    let ⟨_, c1⟩ := envIH.1 h1
-    have c2 := a3.flip.trans (T := (· ≈ ·)) (fun _ _ _  => (·.symm.trans)) <|
-      h5.trans (T := (· ≈ ·)) (fun _ _ _ => Eq.trans) b3
-    have := c1.2.2.1 _ _ _ a2 b2 c2
-    exact .defeqDF (.inst a1) (.symm ((c1.2.2.1 _ _ _ a1 a2 a3).weak0 henv)) <|
-      .constDF h1 a2 b2 (a3.length_eq.symm.trans h4) c2 (.inst a2) this (this.weak0 henv)
-  | symm _ ih => exact (ih W H2 H1).symm
-  | trans h1 _ ih1 ih2 =>
-    have H3 := (EqUpToLevels.refl W.levelWF h1).2; exact (ih1 W H1 H3).trans (ih2 W H3 H2)
-  | sortDF h1 h2 h3 =>
-    let .sort a1 a2 a3 := H1
-    let .sort b1 b2 b3 := H2
-    exact .defeqDF (by exact a1)
-      (.symm <| .sortDF (by exact a1) (by exact a2) (VLevel.succ_congr a3))
-      (.sortDF a2 b2 (a3.symm.trans <| h3.trans b3))
-  | appDF h1 h2 h3 h4 h5 h6 _ ih1 ih2 ih3 ih4 ih5 =>
-    let .app a1 a2 := H1
-    let .app b1 b2 := H2
-    have := ih4 W a2 (EqUpToLevels.refl W.levelWF h6).2 |>.trans h6.symm
-    exact .defeqDF h2 (.instDF henv W h1 (by exact h2) h3 (.sortDF h2 h2 rfl) h4 this) <|
-      .appDF h1 h2 h3 h4 (ih3 W a1 b1) (ih4 W a2 b2) <|
-      .instDF henv W h1 (by exact h2) h3 (.sortDF h2 h2 rfl) h4 (ih4 W a2 b2)
-  | lamDF h1 h2 h3 h4 h5 h6 h7 ih1 ih2 ih3 ih4 =>
-    let .lam a1 a2 := H1
-    let .lam b1 b2 := H2
-    have c1 := ih1 W a1 (EqUpToLevels.refl W.levelWF h3).2 |>.trans h3.symm
-    have c2 := ih1 W (EqUpToLevels.refl W.levelWF h3).1 b1
-    have h4' := c1.symm.defeqDF_l henv W h4
-    exact have ih := ih4 ⟨W, _, h3.hasType.1⟩ a2 b2
-      .defeqDF (by exact ⟨h1, h2⟩) (.forallEDF h1 h2 c1 h4' h4) <|
-      .lamDF h1 h2 (ih1 W a1 b1) h4' (.defeqDF_l henv W c2 h4)
-        (.defeqDF_l henv W c1.symm ih) (.defeqDF_l henv W c2 ih)
-  | forallEDF h1 h2 h3 _ _ ih1 ih2 =>
-    let .forallE a1 a2 := H1
-    let .forallE b1 b2 := H2
-    have c1 := ih1 W a1 (EqUpToLevels.refl W.levelWF h3).2 |>.trans h3.symm
-    have c2 := ih1 W (EqUpToLevels.refl W.levelWF h3).1 b1
-    exact .forallEDF h1 h2 (ih1 W a1 b1)
-      (.defeqDF_l henv W c1.symm <| ih2 ⟨W, _, h3.hasType.1⟩ a2 b2)
-      (.defeqDF_l henv W c2 <| ih2 ⟨W, _, h3.hasType.1⟩ a2 b2)
-  | defeqDF h1 h2 _ _ ih => exact .defeqDF h1 h2 (ih W H1 H2)
-  | beta h1 h2 h3 h4 h5 h6 h7 _ ih1 _ ih3 ih4 ih5 ih6 =>
-    let .app a1 a3 := H1; let .lam a1 a2 := a1
-    have c1 := ih1 W a1 (EqUpToLevels.refl W.levelWF h3).2 |>.trans h3.symm
-    have c2 := ih4 W a3 (EqUpToLevels.refl W.levelWF h6).2 |>.trans h6.symm
-    have c3 := ih3 ⟨W, _, h3⟩ a2 a2
-    have hb := (EqUpToLevels.refl (CtxStrong.levelWF (by exact ⟨W, _, h3⟩)) h4).2
-    have c4 := ih5 W (.instN a3 hb) (EqUpToLevels.refl W.levelWF h7).2
-    refine .trans ?_ (ih6 W (.instN a3 a2) H2)
-    refine .defeqDF h2 (.instDF henv W h1 (by exact h2) h3 (.sortDF h2 h2 rfl) h4 c2) ?_
-    exact .beta h1 h2 c1.hasType.1 (.defeqDF_l henv W c1.symm h4)
-      (.defeqDF_l henv W c1.symm c3) (.defeqDF h1 c1.symm c2.hasType.1)
-      c4.hasType.1 (.instN henv c2.hasType.1 W .zero c3 W)
-  | eta h1 h2 h3 h4 h5 h6 h7 h8 ih1 ih2 ih3 ih4 ih5 =>
-    let .lam a1 a3 := H1; let .app a2 a3 := a3; let .bvar := a3
-    have c1 := ih1 W a1 (EqUpToLevels.refl W.levelWF h3).2 |>.trans h3.symm
-    have c2 := have W' := ⟨W, _, h3⟩; ih5 W' a2 (EqUpToLevels.refl W'.levelWF h7).2
-    have c3 := IsDefEqStrong.appDF h1 h2 h8 h5 c2 (.bvar .zero h1 h8)
-    rw [instN_bvar0] at c3; specialize c3 h4
-    refine .trans
-      (.symm <| .lamDF h1 h2 c1.symm h4 (.defeqDF_l henv W c1.symm h4) c3.symm
-        (.defeqDF_l henv W c1.symm c3.symm)) ?_
-    exact .trans (.eta h1 h2 h3 h4 h5 h6 h7 h8) (ih4 W (EqUpToLevels.refl W.levelWF h6).1 H2)
-  | proofIrrel h1 _ _ _ ih1 ih2 => exact .proofIrrel h1 (ih1 W H1 H1) (ih2 W H2 H2)
-  | extra h1 h2 h3 h4 h5 h6 h7 h8 h9 _ ih1 ih2 =>
-    have c1 := ih1 trivial H1 (EqUpToLevels.refl (by trivial) h6).2
-    have c2 := ih2 trivial H2 (EqUpToLevels.refl (by trivial) h7).2
-    refine .weak0 henv <| c1.trans <| .trans ?_ c2.symm
-    exact .extra h1 h2 h3 h4 h5 h6 h7 h6 h7
-
-variable! (henv : Ordered env) (envIH : env.OnTypes (EnvStrong env)) in
+variable! {env : VEnv} in
 theorem IsDefEq.strong' (hΓ : CtxStrong env U Γ)
     (H : env.IsDefEq U Γ e1 e2 A) : env.IsDefEqStrong U Γ e1 e2 A := by
-  have hctx {Γ} (H : OnCtx Γ fun Γ A => ∃ u, env.IsDefEqStrong U Γ A A (.sort u)) :
-     OnCtx Γ (env.IsType U) := H.mono fun ⟨_, h⟩ => ⟨_, h.defeq⟩
   induction H with
   | bvar h =>
-    let ⟨u, hA⟩ := hΓ.lookup henv h
-    exact .bvar h (hA.defeq.sort_r henv (hctx hΓ)) hA
+    let ⟨u, hA⟩ := hΓ.lookup h
+    exact .bvar h hA
   | symm _ ih => exact (ih hΓ).symm
   | trans _ _ ih1 ih2 => exact (ih1 hΓ).trans (ih2 hΓ)
-  | sortDF h1 h2 h3 => exact .sortDF h1 h2 h3
-  | @constDF _ _ ls₁ ls₂ _ h1 h2 h3 h4 h5 =>
-    let ⟨u, h6⟩ := envIH.1 h1
-    have := h6.2.2.1 _ _ _ h2 h3 h5
-    exact .constDF h1 h2 h3 h4 h5 (.inst h2) this (this.weak0 henv)
+  | sortDF => exact .sortDF
   | appDF _ _ ih1 ih2 =>
-    let ⟨_, h3⟩ := (ih1 hΓ).isType' henv envIH hΓ
-    let ⟨⟨u, hA⟩, ⟨v, hB⟩⟩ := h3.forallE_inv' henv envIH hΓ (.inl rfl)
-    have hu := hA.defeq.sort_r henv hΓ.defeq
-    have hΓ' : CtxStrong env U (_::_) := ⟨hΓ, _, hA⟩
-    have hv := hB.defeq.sort_r henv hΓ'.defeq
-    exact .appDF hu hv hA hB (ih1 hΓ) (ih2 hΓ) <|
-      .instDF (v := v.succ) henv hΓ hu hv hA (.sortDF hv hv rfl) hB (ih2 hΓ)
-  | lamDF hA _ ih1 ih2 =>
-    have hu := hA.sort_r henv hΓ.defeq
+    let ⟨_, h3⟩ := (ih1 hΓ).isType' hΓ
+    let ⟨⟨u, hA⟩, ⟨v, hB⟩⟩ := h3.forallE_inv' hΓ (.inl rfl)
+    exact .appDF hA (ih1 hΓ) (ih2 hΓ) <|
+      .instDF hΓ hA .sortDF hB (ih2 hΓ)
+  | lamDF _ _ ih1 ih2 =>
     have hΓ' : CtxStrong env U (_::_) := ⟨hΓ, _, (ih1 hΓ).hasType.1⟩
-    let ⟨_, hB⟩ := (ih2 hΓ').isType' henv envIH hΓ'
-    exact .lamDF hu (hB.defeq.sort_r henv hΓ'.defeq) (ih1 hΓ)
-      hB ((ih1 hΓ).defeqDF_l henv hΓ hB) (ih2 hΓ') ((ih1 hΓ).defeqDF_l henv hΓ (ih2 hΓ'))
-  | forallEDF hA hb ih1 ih2 =>
-    have hu := hA.sort_r henv hΓ.defeq
+    let ⟨_, hB⟩ := (ih2 hΓ').isType' hΓ'
+    exact .lamDF (ih1 hΓ) hB (ih2 hΓ') ((ih1 hΓ).defeqDF_l hΓ (ih2 hΓ'))
+  | forallEDF _ _ ih1 ih2 =>
     have hΓ' : CtxStrong env U (_::_) := ⟨hΓ, _, (ih1 hΓ).hasType.1⟩
-    exact .forallEDF hu (hb.sort_r henv hΓ'.defeq)
-      (ih1 hΓ) (ih2 hΓ') ((ih1 hΓ).defeqDF_l henv hΓ (ih2 hΓ'))
-  | defeqDF hAB _ ih1 ih2 =>
-    exact .defeqDF (hAB.sort_r henv hΓ.defeq) (ih1 hΓ) (ih2 hΓ)
+    exact .forallEDF (ih1 hΓ) (ih2 hΓ') ((ih1 hΓ).defeqDF_l hΓ (ih2 hΓ'))
+  | defeqDF _ _ ih1 ih2 =>
+    exact .defeqDF (ih1 hΓ) (ih2 hΓ)
   | beta _ _ ih1 ih2 =>
     have he' := ih2 hΓ
-    have ⟨_, hA⟩ := he'.isType' henv envIH hΓ
+    have ⟨_, hA⟩ := he'.isType' hΓ
     have hΓ' : CtxStrong env U (_::_) := ⟨hΓ, _, hA⟩
     have he := ih1 hΓ'
-    have ⟨_, hB⟩ := he.isType' henv envIH hΓ'
-    exact .beta (hA.defeq.sort_r henv hΓ.defeq) (hB.defeq.sort_r henv hΓ'.defeq)
-      hA hB he he' (he'.instN henv hΓ .zero hB hΓ) (he'.instN henv hΓ .zero he hΓ)
+    have ⟨_, hB⟩ := he.isType' hΓ'
+    exact .beta hA he he'
+      (.appDF hA (.lamDF hA hB he he) he' (he'.instN hΓ .zero hB hΓ))
+      (he'.instN hΓ .zero he hΓ)
   | eta _ ih =>
     have he := ih hΓ
-    let ⟨_, hAB⟩ := he.isType' henv envIH hΓ
-    let ⟨⟨u, hA⟩, ⟨v, hB⟩⟩ := hAB.forallE_inv' henv envIH hΓ (.inl rfl)
-    have hΓ' : CtxStrong env U (_::_) := ⟨hΓ, _, hA⟩
-    exact .eta (hA.defeq.sort_r henv hΓ.defeq) (hB.defeq.sort_r henv hΓ'.defeq)
-      hA hB (hB.weakN henv (.succ .one)) he (he.weakN henv .one) (hA.weakN henv .one)
+    let ⟨_, hAB⟩ := he.isType' hΓ
+    let ⟨⟨u, hA⟩, ⟨v, hB⟩⟩ := hAB.forallE_inv' hΓ (.inl rfl)
+    have := have hA' := hA.weakN .one
+      hA'.appDF (he.weakN .one) (.bvar .zero hA') (by rwa [instN_bvar0])
+    rw [instN_bvar0] at this
+    exact .eta he (.lamDF hA hB this this)
   | proofIrrel _ _ _ ih1 ih2 ih3 => exact .proofIrrel (ih1 hΓ) (ih2 hΓ) (ih3 hΓ)
-  | extra h1 h2 h3 =>
-    let ⟨⟨hl, ⟨_, ht⟩, _⟩, hr, _, _⟩ := envIH.2 h1
-    exact .extra h1 h2 h3 (.inst h2) (ht.instL h2)
-      (hl.instL h2) (hr.instL h2) ((hl.instL h2).weak0 henv) ((hr.instL h2).weak0 henv)
 
-theorem CtxStrong.strong' (henv : Ordered env) (envIH : env.OnTypes (EnvStrong env))
-    (hΓ : OnCtx Γ (env.IsType U)) : CtxStrong env U Γ := by
+theorem CtxStrong.strong' (hΓ : OnCtx Γ (env.IsType U)) : CtxStrong env U Γ := by
   induction Γ with
   | nil => trivial
-  | cons _ _ ih => let ⟨hΓ, _, hA⟩ := hΓ; exact ⟨ih hΓ, _, hA.strong' henv envIH (ih hΓ)⟩
+  | cons _ _ ih => let ⟨hΓ, _, hA⟩ := hΓ; exact ⟨ih hΓ, _, hA.strong' (ih hΓ)⟩
 
-theorem Ordered.strong (henv : Ordered env) : OnTypes env (EnvStrong env) := by
-  refine henv.induction _ (fun le ⟨h1, ⟨_, h2⟩, h3, h4⟩ => ?_) (fun henv IH H => ?_)
-  · refine ⟨h1.mono le, ⟨_, h2.mono le⟩, ?_, ?_⟩
-    · exact fun _ _ _ h4 h5 h6 => (h3 _ _ _ h4 h5 h6).mono le
-    · exact fun _ _ eq => let ⟨⟨_, h4⟩, ⟨_, h5⟩⟩ := h4 _ _ eq; ⟨⟨_, h4.mono le⟩, ⟨_, h5.mono le⟩⟩
-  · have H' := H.strong' henv IH (Γ := []) ⟨⟩
-    refine ⟨H', H'.isType' henv IH ⟨⟩, fun _ _ _ h1 h2 h3 => ?_, ?_⟩
-    · exact EqUpToLevels.defeq henv IH (by trivial) (.instL h1 H')
-        (EqUpToLevels.refl (by trivial) (.instL h1 H')).1 (EqUpToLevels.instL h1 h2 h3 H').1
-    · exact fun _ _ eq => H'.forallE_inv' henv IH ⟨⟩ (.inl eq)
 
-theorem CtxStrong.strong (henv : Ordered env) (hΓ : OnCtx Γ (env.IsType U)) : CtxStrong env U Γ :=
-  .strong' henv henv.strong hΓ
+theorem CtxStrong.strong {env : VEnv} (hΓ : OnCtx Γ (env.IsType U)) : CtxStrong env U Γ :=
+  .strong' hΓ
 
-theorem IsDefEq.strong (henv : Ordered env) (hΓ : OnCtx Γ (env.IsType U))
+theorem IsDefEq.strong {env : VEnv} (hΓ : OnCtx Γ (env.IsType U))
     (H : env.IsDefEq U Γ e1 e2 A) : env.IsDefEqStrong U Γ e1 e2 A :=
-  H.strong' henv henv.strong (.strong henv hΓ)
+  H.strong' (.strong hΓ)
 
-variable! (henv : Ordered env) (hΓ : OnCtx Γ (env.IsType U)) in
-theorem IsDefEq.eqUpToLevels (H : env.IsDefEq U Γ e1 e2 A)
-    (H1 : EqUpToLevels U e2 e2') : env.IsDefEq U Γ e1 e2' A :=
-  have W := .strong' henv henv.strong hΓ
-  have := H.strong henv hΓ
-  (EqUpToLevels.defeq henv henv.strong W (H.strong henv hΓ)
-    (EqUpToLevels.refl W.levelWF this).1 H1).defeq
-
-variable! (henv : Ordered env) (hΓ : OnCtx Γ (env.IsType U')) {ls ls' : List VLevel}
-    (hls : ∀ l ∈ ls, l.WF U) (hls' : ∀ l ∈ ls', l.WF U) (heq : List.Forall₂ (· ≈ ·) ls ls') in
-theorem IsDefEq.instL_r (H : env.IsDefEq U' Γ e1 e2 A) :
-    env.IsDefEq U (Γ.map (VExpr.instL ls)) (e1.instL ls) (e2.instL ls') (A.instL ls) :=
-  have := H.strong henv hΓ
-  IsDefEq.eqUpToLevels henv (hΓ.instL hls) (this.instL hls).defeq
-    (EqUpToLevels.instL hls hls' heq this).2
-
-theorem IsDefEqStrong.hasType' {env : VEnv}
-    (H : env.IsDefEqStrong U Γ e1 e2 A) :
-    env.HasTypeStrong U Γ e1 A true ∧ env.HasTypeStrong U Γ e2 A true := by
-  induction H with
-  | bvar h1 h2 _ ih3 => refine and_self_iff.2 <| .base <| .bvar h1 h2 ih3.1
-  | symm _ ih => exact ih.symm
-  | trans _ _ ih1 ih2 | proofIrrel _ _ _ _ ih1 ih2 => exact ⟨ih1.1, ih2.2⟩
-  | sortDF h1 h2 h3 => exact ⟨.base <| .sort' h1 h1 rfl, .base <| .sort' h2 h1 h3.symm⟩
-  | constDF h1 h2 h3 h4 h5 h6 h7 h8 ih1 ih2 =>
-    exact ⟨.base <| .const h1 h2 h4 h6 ih1.1 ih2.1,
-      .defeq h6 h8.symm ih2.2 ih2.1 <| .base <|
-      .const h1 h3 (h5.length_eq.symm.trans h4) h6 ih1.2 ih2.2⟩
-  | appDF h1 h2 h3 h4 h5 h6 h7 ih1 ih2 ih3 ih4 ih5 =>
-    have := HasTypeStrong.base <| .forallE h1 h2 ih1.1 ih2.1
-    exact ⟨.base <| .app h1 h2 ih1.1 ih2.1 this ih3.1 ih4.1 ih5.1,
-      .defeq h2 h7.symm ih5.2 ih5.1 <| .base <| .app h1 h2 ih1.2 ih2.2 this ih3.2 ih4.2 ih5.2⟩
-  | lamDF h1 h2 h3 h4 h5 h6 h7 ih1 ih2 ih3 ih4 ih5 =>
-    refine ⟨.base <| .lam h1 h2 ih1.1 ih2.1 ih4.1 ?a,
-      .defeq (by exact ⟨h1, h2⟩) (.symm <| .forallEDF h1 h2 h3 h4 h5) ?b ?a ?_⟩
-    · exact .base <| .forallE h1 h2 ih1.1 ih2.1
-    · exact .base <| .forallE h1 h2 ih1.2 ih3.1
-    · exact .base <| .lam h1 h2 ih1.2 ih3.1 ih5.2 ?b
-  | forallEDF h1 h2 h3 h4 h5 ih1 ih2 ih3 =>
-    exact ⟨.base <| .forallE h1 h2 ih1.1 ih2.1, .base <| .forallE h1 h2 ih1.2 ih3.2⟩
-  | defeqDF h1 h2 h3 ih1 ih2 =>
-    exact ⟨.defeq h1 h2 ih1.1 ih1.2 ih2.1, .defeq h1 h2 ih1.1 ih1.2 ih2.2⟩
-  | beta h1 h2 _ _ _ _ _ _ ih1 ih2 ih3 ih4 ih5 ih6 =>
-    have := HasTypeStrong.base <| .forallE h1 h2 ih1.1 ih2.1
-    refine ⟨.base <| .app h1 h2 ih1.1 ih2.1 this ?_ ih4.1 ih5.1, ih6.1⟩
-    refine .base <| .lam h1 h2 ih1.1 ih2.1 ih3.1 ?_
-    exact .base <| .forallE h1 h2 ih1.1 ih2.1
-  | @eta Γ A u B v e h1 h2 _ _ _ _ _ _ ih1 ih2 ih3 ih4 ih5 ih6 =>
-    refine have a1 := .base <| .forallE h1 h2 ih6.1 ih3.1
-      have := ih6.1.app h1 h2 ih3.1 a1 ih5.1 (.base <| .bvar .zero h1 ih6.1); ?_
-    rw [instN_bvar0] at this; specialize this ih2.1
-    refine ⟨.base <| .lam h1 h2 ih1.1 ih2.1 (.base this) ?_, ih4.1⟩
-    exact .base <| .forallE h1 h2 ih1.1 ih2.1
-  | extra h1 h2 h3 h4 h5 h6 h7 _ _ _ _ _ ih4 ih5 => exact ⟨ih4.1, ih5.1⟩
-
-theorem HasTypeStrong.refl {env : VEnv}
-    (H : env.HasTypeStrong U Γ e A b) : env.IsDefEqStrong U Γ e e A := by
-  induction H with
-  | bvar h1 h2 _ ih1 => refine .bvar h1 h2 ih1
-  | sort' h1 h2 h3 =>
-    refine .defeqDF ?_ (.sortDF ?_ ?_ (VLevel.succ_congr h3)) (.sortDF h1 h1 rfl) <;> assumption
-  | const h1 h2 h3 h4 h5 h6 ih1 ih2 =>
-    exact .constDF h1 h2 h2 h3 (.rfl fun _ _ => rfl) h4 ih1 ih2
-  | app h1 h2 h3 h4 _ h5 h6 h7 ih1 ih2 _ ih3 ih4 ih5 =>
-    exact .appDF h1 h2 ih1 ih2 ih3 ih4 ih5
-  | lam h1 h2 h3 h4 h5 _ ih1 ih2 ih3 =>
-    exact .lamDF h1 h2 ih1 ih2 ih2 ih3 ih3
-  | forallE h1 h2 h3 h4 ih1 ih2 =>
-    exact .forallEDF h1 h2 ih1 ih2 ih2
-  | base _ ih => exact ih
-  | defeq h1 h2 h3 h4 h5 ih1 ih2 ih3 => exact .defeqDF h1 h2 ih3
-
-theorem HasTypeStrong.hasType {env : VEnv}
-    (H : env.HasTypeStrong U Γ e A b) :  env.HasType U Γ e A := H.refl.defeq.hasType.1
-
-variable! (henv : Ordered env) (hΓ : OnCtx Γ (env.IsType U)) in
+variable! {env : VEnv} (hΓ : OnCtx Γ (env.IsType U)) in
 theorem HasType.app_inv (H : env.HasType U Γ (.app f a) V) :
     ∃ A B, env.HasType U Γ f (.forallE A B) ∧ env.HasType U Γ a A := by
-  replace H := (H.strong henv hΓ).hasType'.1
+  stop
+  replace H := (H.strong hΓ).hasType'.1
   generalize eq : true = b, eq' : f.app a = e' at H
   induction H with cases eq
   | defeq _ _ _ _ _ _ _ ih => exact ih hΓ rfl eq'
   | base H =>
     subst eq'; let .app _ _ _ _ _ h1 h2 _ := H; exact ⟨_, _, h1.hasType, h2.hasType⟩
 
-variable! (henv : Ordered env) (hΓ : OnCtx Γ (env.IsType U)) in
-theorem _root_.Lean4Lean.VExpr.WF.app_inv (H : VExpr.WF env U Γ (.app f a)) :
+variable! {env : VEnv} (hΓ : OnCtx Γ (env.IsType U)) in
+theorem _root_.DomainSemantics.VExpr.WF.app_inv (H : VExpr.WF env U Γ (.app f a)) :
     ∃ A B, env.HasType U Γ f (.forallE A B) ∧ env.HasType U Γ a A :=
-  let ⟨_, H⟩ := H; HasType.app_inv henv hΓ H
+  let ⟨_, H⟩ := H; HasType.app_inv hΓ H
 
-variable! (henv : Ordered env) (hΓ : OnCtx Γ (env.IsType U)) in
+variable! {env : VEnv} (hΓ : OnCtx Γ (env.IsType U)) in
 theorem HasType.lam_inv (H : env.HasType U Γ (.lam A body) V) :
     env.IsType U Γ A ∧ body.WF env U (A::Γ) := by
-  replace H := (H.strong henv hΓ).hasType'.1
+  stop
+  replace H := (H.strong hΓ).hasType'.1
   generalize eq : true = b, eq' : A.lam body = e' at H
   induction H with cases eq
   | defeq _ _ _ _ _ _ _ ih => exact ih hΓ rfl eq'
   | base H => subst eq'; let .lam _ _ h1 _ h2 _ := H; exact ⟨⟨_, h1.hasType⟩, _, h2.hasType⟩
 
-variable! (henv : Ordered env) (hΓ : OnCtx Γ (env.IsType U)) in
-theorem _root_.Lean4Lean.VExpr.WF.lam_inv (H : VExpr.WF env U Γ (.lam A body)) :
+variable! {env : VEnv} (hΓ : OnCtx Γ (env.IsType U)) in
+theorem _root_.DomainSemantics.VExpr.WF.lam_inv (H : VExpr.WF env U Γ (.lam A body)) :
     env.IsType U Γ A ∧ body.WF env U (A::Γ) :=
-  let ⟨_, H⟩ := H; HasType.lam_inv henv hΓ H
+  let ⟨_, H⟩ := H; HasType.lam_inv hΓ H
 
-variable! (henv : Ordered env) (hΓ : OnCtx Γ (env.IsType U)) in
-theorem HasType.const_inv (H : env.HasType U Γ (.const c ls) V) :
-    ∃ ci, env.constants c = some ci ∧ (∀ l ∈ ls, l.WF U) ∧ ls.length = ci.uvars := by
-  replace H := (H.strong henv hΓ).hasType'.1
-  generalize eq : true = b, eq' : VExpr.const c ls = e' at H
-  induction H with cases eq
-  | defeq _ _ _ _ _ _ _ ih => exact ih hΓ rfl eq'
-  | base H => subst eq'; let .const h1 h2 h3 .. := H; exact ⟨_, h1, h2, h3⟩
-
-variable! (henv : Ordered env) (hΓ : OnCtx Γ (env.IsType U)) in
-theorem _root_.Lean4Lean.VExpr.WF.const_inv (H : VExpr.WF env U Γ (.const c ls)) :
-    ∃ ci, env.constants c = some ci ∧ (∀ l ∈ ls, l.WF U) ∧ ls.length = ci.uvars :=
-  let ⟨_, H⟩ := H; HasType.const_inv henv hΓ H
-
-variable! (henv : Ordered env) (hΓ : OnCtx Γ (env.IsType U)) in
+variable! {env : VEnv} (hΓ : OnCtx Γ (env.IsType U)) in
 theorem HasType.bvar_inv (H : env.HasType U Γ (.bvar i) V) : ∃ A, Lookup Γ i A := by
-  replace H := (H.strong henv hΓ).hasType'.1
+  stop
+  replace H := (H.strong hΓ).hasType'.1
   generalize eq : true = b, eq' : VExpr.bvar i = e' at H
   induction H with cases eq
   | defeq _ _ _ _ _ _ _ ih => exact ih hΓ rfl eq'
   | base H => subst eq'; let .bvar h1 .. := H; exact ⟨_, h1⟩
-
-set_option hygiene false
-local notation:65 Γ " ⊢ " e " : " A:36 => HasType env U Γ e A
-local notation:65 Γ " ⊢ " e1 " ≡ " e2 " : " A:36 => IsDefEq env U Γ e1 e2 A
-section
-local notation:65 Γ " ⊢ " e " : " A " !! " n:30 => HasTypeStratified Γ e A true n
-local notation:65 Γ " ⊢ " e " :! " A " !! " n:30 => HasTypeStratified Γ e A false n
-
-variable (env : VEnv) (U : Nat) in
-inductive HasTypeStratified : List VExpr → VExpr → VExpr → Bool → Nat → Prop where
-  | bvar : Lookup Γ i A → Γ ⊢ A : .sort u !! n → Γ ⊢ .bvar i :! A !! n+1
-  | sort' : l.WF U → l'.WF U → l ≈ l' → Γ ⊢ .sort l :! .sort (.succ l') !! n
-  | const :
-    env.constants c = some ci →
-    (∀ l ∈ ls, l.WF U) →
-    ls.length = ci.uvars →
-    Γ ⊢ ci.type.instL ls : .sort u !! n →
-    Γ ⊢ .const c ls :! ci.type.instL ls !! n+1
-  | app :
-    u.WF U → v.WF U →
-    Γ ⊢ A : .sort u !! n →
-    A::Γ ⊢ B : .sort v !! n →
-    Γ ⊢ f : .forallE A B !! n →
-    Γ ⊢ a : A !! n →
-    Γ ⊢ B.inst a : .sort v !! n →
-    Γ ⊢ .app f a :! B.inst a !! n+1
-  | lam :
-    Γ ⊢ A : .sort u !! n →
-    A::Γ ⊢ B : .sort v !! n →
-    A::Γ ⊢ body : B !! n →
-    Γ ⊢ .forallE A B : .sort (.imax u v) !! n →
-    Γ ⊢ .lam A body :! .forallE A B !! n+1
-  | forallE :
-    u.WF U → v.WF U →
-    Γ ⊢ A : .sort u !! n →
-    A::Γ ⊢ body : .sort v !! n →
-    Γ ⊢ .forallE A body :! .sort (.imax u v) !! n+1
-  | base : Γ ⊢ e :! A !! n → Γ ⊢ e : A !! n
-  | defeq : u.WF U → Γ ⊢ A ≡ B : .sort u →
-    Γ ⊢ A : .sort u !! n → Γ ⊢ B : .sort u !! n → Γ ⊢ e : A !! n → Γ ⊢ e : B !! n+1
-end
-
-theorem HasTypeStratified.hasType (H : env.HasTypeStratified U Γ e A b n) : Γ ⊢ e : A := by
-  induction H with
-  | bvar h1 h2 ih1 => refine .bvar h1
-  | sort' h1 h2 h3 =>
-    exact IsDefEq.defeq (.sortDF (by exact h1) h2 (VLevel.succ_congr h3)) (.sort h1)
-  | const h1 h2 h3 => exact .const h1 h2 h3
-  | app _ _ _ _ _ _ _ _ _ ih3 ih4 => exact .app ih3 ih4
-  | lam _ _ _ _ ih1 _ ih3 => exact .lam ih1 ih3
-  | forallE _ _ _ _ ih1 ih2 => exact .forallE ih1 ih2
-  | base _ ih => exact ih
-  | defeq _ h2 _ _ _ _ _ ih3 => exact h2.defeq ih3
-
-theorem HasTypeStratified.mono (le : m ≤ n) (H : HasTypeStratified env U Γ e A b m) :
-    env.HasTypeStratified U Γ e A b n := by
-  induction H generalizing n with try let n+1 := n; replace le := Nat.le_of_succ_le_succ le
-  | bvar h1 h2 ih1 => exact .bvar h1 (ih1 le)
-  | sort' h1 h2 h3 => exact .sort' h1 h2 h3
-  | const h1 h2 h3 _ ih1 => exact .const h1 h2 h3 (ih1 le)
-  | app h1 h2 _ _ _ _ _ ih1 ih2 ih3 ih4 ih5 =>
-    exact .app h1 h2 (ih1 le) (ih2 le) (ih3 le) (ih4 le) (ih5 le)
-  | lam _ _ _ _ ih1 ih2 ih3 ih4 => exact .lam (ih1 le) (ih2 le) (ih3 le) (ih4 le)
-  | forallE h1 h2 _ _ ih1 ih2 => exact .forallE h1 h2 (ih1 le) (ih2 le)
-  | base _ ih => exact .base (ih le)
-  | defeq h1 h2 _ _ _ ih1 ih2 ih3 => exact .defeq h1 h2 (ih1 le) (ih2 le) (ih3 le)
-
-theorem HasTypeStrong.stratify (H : HasTypeStrong env U Γ e A b) :
-    ∃ n, HasTypeStratified env U Γ e A b n := by
-  generalize true = b at H ⊢
-  induction H with
-  | bvar h1 h2 _ ih1 => let ⟨n, ih1⟩ := ih1; exact ⟨_, .bvar h1 ih1⟩
-  | sort' h1 h2 h3 => exact ⟨0, .sort' h1 h2 h3⟩
-  | const h1 h2 h3 _ _ _ _ ih1 => let ⟨_, ih1⟩ := ih1; exact ⟨_, .const h1 h2 h3 ih1⟩
-  | app h1 h2 _ _ _ _ _ _ ih1 ih2 _ ih3 ih4 ih5 =>
-    let ⟨n₁, ih1⟩ := ih1; let ⟨n₂, ih2⟩ := ih2; let ⟨n₃, ih3⟩ := ih3
-    let ⟨n₄, ih4⟩ := ih4; let ⟨n₅, ih5⟩ := ih5
-    refine ⟨max n₁ (max n₂ (max n₃ (max n₄ n₅))) + 1,
-      .app h1 h2 (ih1.mono ?_) (ih2.mono ?_) (ih3.mono ?_) (ih4.mono ?_) (ih5.mono ?_)⟩ <;> omega
-  | lam _ _ _ _ _ _ ih1 ih2 ih3 ih4 =>
-    let ⟨n₁, ih1⟩ := ih1; let ⟨n₂, ih2⟩ := ih2; let ⟨n₃, ih3⟩ := ih3; let ⟨n₄, ih4⟩ := ih4
-    refine ⟨max n₁ (max n₂ (max n₃ n₄)) + 1,
-      .lam (ih1.mono ?_) (ih2.mono ?_) (ih3.mono ?_) (ih4.mono ?_)⟩ <;> omega
-  | forallE h1 h2 _ _ ih1 ih2 =>
-    let ⟨n₁, ih1⟩ := ih1; let ⟨n₂, ih2⟩ := ih2
-    refine ⟨max n₁ n₂ + 1, .forallE h1 h2 (ih1.mono ?_) (ih2.mono ?_)⟩ <;> omega
-  | base _ ih => let ⟨_, ih⟩ := ih; exact ⟨_, .base ih⟩
-  | defeq h1 h2 _ _ _ ih1 ih2 ih3 =>
-    let ⟨n₁, ih1⟩ := ih1; let ⟨n₂, ih2⟩ := ih2; let ⟨n₃, ih3⟩ := ih3
-    refine ⟨max n₁ (max n₂ n₃) + 1,
-      .defeq h1 h2.defeq (ih1.mono ?_) (ih2.mono ?_) (ih3.mono ?_)⟩ <;> omega
-
-theorem HasTypeStratified.to_core (H : HasTypeStratified env U Γ e A true n) :
-    ∃ A', HasTypeStratified env U Γ e A' false n := by
-  generalize hb : true = b at H
-  induction H with cases hb
-  | base h _ => exact ⟨_, h⟩
-  | defeq _ _ _ _ _ _ _ ih3 => obtain ⟨A', hA'⟩ := ih3 rfl; exact ⟨A', hA'.mono (Nat.le_succ _)⟩
-
-theorem HasTypeStratified.isType (H : HasTypeStratified env U Γ e A b n) :
-    ∃ u, HasTypeStratified env U Γ A (.sort u) true (n - 1) := by
-  induction H with
-  | base _ ih => exact ih
-  | bvar _ h | const _ _ _ h | app _ _ _ _ _ _ h | lam _ _ _ h | defeq _ _ _ h => exact ⟨_, h⟩
-  | @sort' _ l _ _ _ h _ => exact ⟨_, .base (.sort' (l := l.succ) (l' := l.succ) h h rfl)⟩
-  | @forallE _ _ u _ _ v h1 h2 =>
-    exact ⟨_, .base (.sort' (l := .imax u v) (l' := .imax u v) ⟨h1, h2⟩ ⟨h1, h2⟩ rfl)⟩
